theories/Syntax/FunDecl.v
@@ -40,7 +40,6 @@ Module Type FunDeclKit (Import T : Types).
 
   (* Names of functions. *)
   Parameter Inline 𝑭 : PCtx -> Ty -> Set.
-  #[export] Declare Instance 𝑭_eq_dec : EqDec (sigT (fun Γ => sigT (𝑭 Γ))).
   Parameter Inline 𝑭𝑿 : PCtx -> Ty -> Set.
   (* Names of lemmas. *)
   Parameter Inline 𝑳 : PCtx -> Set.
